lean-fx-2/LeanFX2/Smoke/AuditTypedInversion.lean
@@ -534,5 +534,6 @@ namespace LeanFX2.SmokeTypedInversion
 #print axioms LeanFX2.Term.partialStrengthenTyped?_atNatZero_imp_sound
 #print axioms LeanFX2.Term.partialStrengthenTyped?_atInterval0_imp_sound
 #print axioms LeanFX2.Term.partialStrengthenTyped?_atInterval1_imp_sound
+#print axioms LeanFX2.Term.partialStrengthenTyped?_atVar_imp_sound
 
 end LeanFX2.SmokeTypedInversion
